LambdaLab/Parser/Token.lean
@@ -1,6 +1,0 @@
-
-namespace LambdaLab.Parser
-
-abbrev Restricted (P : String → Prop) : Type := { s : String // P s }
-
-end LambdaLab.Parser
