LambdaLab/ParserOld/Token.lean
@@ -1,0 +1,6 @@
+
+namespace LambdaLab.ParserOld
+
+abbrev Restricted (P : String → Prop) : Type := { s : String // P s }
+
+end LambdaLab.ParserOld
